README.md
@@ -1,2 +1,15 @@
 # Extended Proof Rules
- Proof soundness of some extended proof rules
+Proof soundness of some extended proof rules
+
+# Installation
+0. The project requires Coq 8.15.2.
+1. Run ```coq_makefile -f _CoqProject -o Makefile``` to generate a Makefile that will work on your machine.
+2. Run ```make``` to compile the project.
+
+# Table of Content
+- Imp.v: Basic imperative language
+- ImpCF.v: Extension of the imperative language with control flow support
+- Embeddings.v: Definitions of three shallow embeddings (big-step based embedding, weakest precondition based embedding, and continuation based embedding)
+- BigSProof.v: Proofs of extended rules in big-step based embedding
+- SmallSProof.v: Proofs of extended rules in weakest precondition based embedding
+- ContProof.v: Proofs of extended rules in continuation based embedding
